Drop division, focus on multiplication
I think doing division properly requires exposing more operators
in asmScript, so that it can be consistently signed or unsigned
across platforms.

I'm fine with using software division for oddball targets,
but for ARMv8 and x86 I'd really like to target a division
instruction.

pancake/crep_to_loopScript.sml
@@ -42,58 +42,12 @@ Definition prog_if_def:
     (Assign n (Const 1w)) (Assign n (Const 0w)) (list_insert [n; m] l)]
 End
 
-(* The following code is based on the fact that the code in
-   data_to_wordTheory.LongDiv1_code is based on
-   multiwordTheory.single_div_loop_def *)
-Definition loop_div_def:
-  loop_div m n tmp l =
-  let l = insert tmp () $ insert (tmp+1) () $ insert (tmp+2) () $ insert (tmp+3) () l in
-    ([Assign tmp (Const (n2w(dimindex(:'a)):'a word)); (* k *)
-      Assign (tmp+1) (Var n); (* ns *)
-      Assign (tmp+2) (Const 0w); (* m *)
-      Assign (tmp+3) (Var m); (* is *)
-      Loop l
-           (If Equal tmp (Imm 0w) Break
-            (Seq
-             (Assign (tmp+1) $ Shift Lsr (Var $ tmp+1) 1) $ Seq
-             (Assign (tmp+1) $ Shift Lsl (Var $ tmp+2) 1) $
-             If Equal (tmp+1) (Reg $ tmp+3)
-             (Assign tmp (Op Sub [Var tmp; Const 1w]))
-             (Seq
-              (Assign (tmp+2) (Op Add [Var $ tmp+2; Const 1w])) $ Seq
-              (Assign (tmp+3) (Op Sub [Var $ tmp+3; Var $ tmp+1])) $
-              Assign tmp (Op Add [Var tmp;Const 1w]))
-             l)
-            l)
-           l;
-     Assign (tmp+3) (Var $ tmp + 2)],tmp+3)
-End
-
 Definition compile_crepop_def:
-  (compile_crepop crepLang$Div target x y tmp l =
-  if target = x86_64 then
-    ([Assign tmp (Const 0w);Arith (LLongDiv (tmp+1) tmp tmp x y)],tmp+1)
-  else if target = ARMv8 ∨ target = MIPS ∨ target = RISC_V then
-    ([Arith (LDiv tmp x y)],tmp)
-  else
-    loop_div x y tmp l) ∧
   (compile_crepop crepLang$Mul target x y tmp l =
   if target = ARMv7 then
-    ([Arith (LLongMul (tmp+1) tmp x y)],tmp+1)
+    ([Arith (LLongMul tmp (tmp+1) x y)],tmp+1)
   else
-    ([Arith (LLongMul tmp tmp x y)],tmp)) ∧
-  compile_crepop crepLang$Mod target x y tmp l =
-  if target = x86_64 then
-    ([Assign tmp (Const 0w);Arith (LLongDiv tmp (tmp+1) tmp x y)],tmp+1)
-  else if target = ARMv8 ∨ target = MIPS ∨ target = RISC_V then
-    ([Arith (LDiv (tmp+2) x y);
-      Assign (tmp+1) (Const 0w);
-      Arith (LLongMul tmp (tmp+1) (tmp+2) y);
-      Assign (tmp+2) (Op Sub [Var x;Var tmp])
-     ],tmp+2)
-  else
-    (* TODO: what is sensible behaviour here? *)
-    ([Assign tmp (Const 0w)],tmp)
+    ([Arith (LLongMul tmp tmp x y)],tmp))
 End
 
 Definition compile_exp_def:
@@ -111,9 +65,9 @@ Definition compile_exp_def:
   (compile_exp ctxt tmp l (Op bop es) =
    let (p, les, tmp, l) = compile_exps ctxt tmp l es in
    (p, Op bop les, tmp, l)) /\
-  (compile_exp ctxt tmp l (Crepop cop es) =
-   let (p, les, tmp, l) = compile_exps ctxt tmp l es;
-       (p',tmp') = compile_crepop cop ctxt.target (tmp) (tmp+1) (tmp+LENGTH les) l
+  (compile_exp ctxt tmp'' l (Crepop cop es) =
+   let (p, les, tmp, l) = compile_exps ctxt tmp'' l es;
+       (p',tmp') = compile_crepop cop ctxt.target (tmp) (tmp+1) (tmp+LENGTH les) $ list_insert (GENLIST ($+ tmp) (LENGTH les)) l
     in
    (p ++ MAPi (λn. Assign (tmp+n)) les ++ p',
     Var tmp', tmp'+1, insert tmp' () $ list_insert (GENLIST ($+ tmp) (tmp'-tmp)) l)) /\
